rename Exp → Exponential

Arithmetization/IDeltaZero/Exponential/Exp.lean
@@ -53,20 +53,20 @@ lemma ext_rem {i j z : M} (ppi : PPow2 i) (ppj : PPow2 j) (hij : i < j) : ext i 
     ext i (z % j) = ext i (j * (z / j) + (z % j)) := by symm; exact ext_add_of_dvd_sq_left ppi.pos (Dvd.dvd.mul_right this (z / j))
     _               = ext i z                          := by simp [div_add_mod]
 
-def Exp.Seq₀ (X Y : M) : Prop := ext 4 X = 1 ∧ ext 4 Y = 2
+def Exponential.Seq₀ (X Y : M) : Prop := ext 4 X = 1 ∧ ext 4 Y = 2
 
-def Exp.Seqₛ.Even (X Y u : M) : Prop := ext (u^2) X = 2 * ext u X ∧ ext (u^2) Y = (ext u Y)^2
+def Exponential.Seqₛ.Even (X Y u : M) : Prop := ext (u^2) X = 2 * ext u X ∧ ext (u^2) Y = (ext u Y)^2
 
-def Exp.Seqₛ.Odd (X Y u : M) : Prop := ext (u^2) X = 2 * ext u X + 1 ∧ ext (u^2) Y = 2 * (ext u Y)^2
+def Exponential.Seqₛ.Odd (X Y u : M) : Prop := ext (u^2) X = 2 * ext u X + 1 ∧ ext (u^2) Y = 2 * (ext u Y)^2
 
-def Exp.Seqₛ (y X Y : M) : Prop := ∀ u ≤ y, u ≠ 2 → PPow2 u → Seqₛ.Even X Y u ∨ Seqₛ.Odd X Y u
+def Exponential.Seqₛ (y X Y : M) : Prop := ∀ u ≤ y, u ≠ 2 → PPow2 u → Seqₛ.Even X Y u ∨ Seqₛ.Odd X Y u
 
-def Exp.Seqₘ (x y X Y : M) : Prop := ∃ u ≤ y^2, u ≠ 2 ∧ PPow2 u ∧ ext u X = x ∧ ext u Y = y
+def Exponential.Seqₘ (x y X Y : M) : Prop := ∃ u ≤ y^2, u ≠ 2 ∧ PPow2 u ∧ ext u X = x ∧ ext u Y = y
 
-def Exp (x y : M) : Prop := (x = 0 ∧ y = 1) ∨ ∃ X ≤ y^4, ∃ Y ≤ y^4, Exp.Seq₀ X Y ∧ Exp.Seqₛ y X Y ∧ Exp.Seqₘ x y X Y
+def Exponential (x y : M) : Prop := (x = 0 ∧ y = 1) ∨ ∃ X ≤ y^4, ∃ Y ≤ y^4, Exponential.Seq₀ X Y ∧ Exponential.Seqₛ y X Y ∧ Exponential.Seqₘ x y X Y
 
-lemma Exp.Seqₛ.iff (y X Y : M) :
-  Exp.Seqₛ y X Y ↔
+lemma Exponential.Seqₛ.iff (y X Y : M) :
+  Exponential.Seqₛ y X Y ↔
   ∀ u ≤ y, u ≠ 2 → PPow2 u →
     ((∃ ext_u_X ≤ X, ext_u_X = ext u X ∧ 2 * ext_u_X = ext (u^2) X)     ∧ (∃ ext_u_Y ≤ Y, ext_u_Y = ext u Y ∧ ext_u_Y^2 = ext (u^2) Y)) ∨
     ((∃ ext_u_X ≤ X, ext_u_X = ext u X ∧ 2 * ext_u_X + 1 = ext (u^2) X) ∧ (∃ ext_u_Y ≤ Y, ext_u_Y = ext u Y ∧ 2 * ext_u_Y^2 = ext (u^2) Y)) :=
@@ -79,22 +79,22 @@ lemma Exp.Seqₛ.iff (y X Y : M) :
       · exact Or.inl ⟨by simp [hx, hy], by simp [hx, hy]⟩
       · exact Or.inr ⟨by simp [hx, hy], by simp [hx, hy]⟩⟩
 
-def Exp.Seqₛ.def : Δ₀-Sentence 3 := ⟨
+def Exponential.Seqₛ.def : Δ₀-Sentence 3 := ⟨
   “∀[#0 < #1 + 1](#0 ≠ 2 → !ppow2Def [#0] →
     ( ∃[#0 < #3 + 1] (!extDef [#0, #1, #3] ∧ !extDef [2 * #0, #1 * #1, #3]) ∧
       ∃[#0 < #4 + 1] (!extDef [#0, #1, #4] ∧ !extDef [#0 * #0, #1 * #1, #4]) ) ∨
     ( ∃[#0 < #3 + 1] (!extDef [#0, #1, #3] ∧ !extDef [2 * #0 + 1, #1 * #1, #3]) ∧
       ∃[#0 < #4 + 1] (!extDef [#0, #1, #4] ∧ !extDef [2 * (#0 * #0), #1 * #1, #4])))”, by simp⟩
 
-lemma Exp.Seqₛ.defined : Δ₀-Relation₃ (Exp.Seqₛ : M → M → M → Prop) via Exp.Seqₛ.def := by
-  intro v; simp [Exp.Seqₛ.iff, Exp.Seqₛ.def, ppow2_defined.pval,
+lemma Exponential.Seqₛ.defined : Δ₀-Relation₃ (Exponential.Seqₛ : M → M → M → Prop) via Exponential.Seqₛ.def := by
+  intro v; simp [Exponential.Seqₛ.iff, Exponential.Seqₛ.def, ppow2_defined.pval,
     ext_defined.pval, ←le_iff_lt_succ, sq, numeral_eq_natCast]
 
-lemma Exp.graph_iff (x y : M) :
-    Exp x y ↔
+lemma Exponential.graph_iff (x y : M) :
+    Exponential x y ↔
     (x = 0 ∧ y = 1) ∨ ∃ X ≤ y^4, ∃ Y ≤ y^4,
       (1 = ext 4 X ∧ 2 = ext 4 Y) ∧
-      Exp.Seqₛ y X Y ∧
+      Exponential.Seqₛ y X Y ∧
       (∃ u ≤ y^2, u ≠ 2 ∧ PPow2 u ∧ x = ext u X ∧ y = ext u Y) :=
   ⟨by rintro (H | ⟨X, bX, Y, bY, H₀, Hₛ, ⟨u, hu, ne2, ppu, hX, hY⟩⟩)
       · exact Or.inl H
@@ -103,20 +103,20 @@ lemma Exp.graph_iff (x y : M) :
       · exact Or.inl H
       · exact Or.inr ⟨X, bX, Y, bY, ⟨H₀.1.symm, H₀.2.symm⟩, Hₛ, ⟨u, hu, ne2, ppu, hX.symm, hY.symm⟩⟩⟩
 
-def Exp.def : Δ₀-Sentence 2 := ⟨
+def Exponential.def : Δ₀-Sentence 2 := ⟨
   “(#0 = 0 ∧ #1 = 1) ∨ (
     ∃[#0 < #2 * #2 * #2 * #2 + 1] ∃[#0 < #3 * #3 * #3 * #3 + 1] (
       (!extDef [1, 4, #1] ∧ !extDef [2, 4, #0]) ∧
-      !Exp.Seqₛ.def [#3, #1, #0] ∧
+      !Exponential.Seqₛ.def [#3, #1, #0] ∧
       ∃[#0 < #4 * #4 + 1] (#0 ≠ 2 ∧ !ppow2Def [#0] ∧ !extDef [#3, #0, #2] ∧!extDef [#4, #0, #1])))”, by simp⟩
 
-lemma Exp.defined : Δ₀-Relation (Exp : M → M → Prop) via Exp.def := by
-  intro v; simp [Exp.graph_iff, Exp.def, ppow2_defined.pval, ext_defined.pval,
-    Exp.Seqₛ.defined.pval, ←le_iff_lt_succ, pow_four, sq, numeral_eq_natCast]
+lemma Exponential.defined : Δ₀-Relation (Exponential : M → M → Prop) via Exponential.def := by
+  intro v; simp [Exponential.graph_iff, Exponential.def, ppow2_defined.pval, ext_defined.pval,
+    Exponential.Seqₛ.defined.pval, ←le_iff_lt_succ, pow_four, sq, numeral_eq_natCast]
 
-instance exp_definable : DefinableRel ℒₒᵣ Σ 0 (Exp : M → M → Prop) := defined_to_with_param _ Exp.defined
+instance exponential_definable : DefinableRel ℒₒᵣ Σ 0 (Exponential : M → M → Prop) := defined_to_with_param _ Exponential.defined
 
-namespace Exp
+namespace Exponential
 
 def seqX₀ : M := 4
 
@@ -187,9 +187,9 @@ lemma Seqₛ.append {z x y X Y i : M} (h : Seqₛ z X Y) (ppi : PPow2 i) (hz : z
   · right; rw [ext_append_of_lt, ext_append_of_lt, ext_append_of_lt, ext_append_of_lt] <;> try simp [ppi.sq, ppj.sq, lt_of_le_of_lt hj hz, *]
     exact H
 
-@[simp] lemma exp_zero_one : Exp (0 : M) 1 := Or.inl (by simp)
+@[simp] lemma exponential_zero_one : Exponential (0 : M) 1 := Or.inl (by simp)
 
-@[simp] lemma exp_one_two : Exp (1 : M) 2 :=
+@[simp] lemma exponential_one_two : Exponential (1 : M) 2 :=
   Or.inr ⟨
     4, by simp [pow_four_eq_sq_sq, two_pow_two_eq_four],
     2 * 4, by simp [pow_four_eq_sq_sq, two_pow_two_eq_four, sq (4 : M)]; exact le_of_lt two_lt_four,
@@ -197,7 +197,7 @@ lemma Seqₛ.append {z x y X Y i : M} (h : Seqₛ z X Y) (ppi : PPow2 i) (hz : z
     by simp [Seqₛ]; intro i hi ne2 ppi; exact False.elim <| not_le.mpr (ppi.two_lt ne2) hi,
     ⟨4, by simp [two_pow_two_eq_four], by simp, by simp [ext, one_lt_four, two_lt_four]⟩⟩
 
-lemma pow2_ext_of_seq₀_of_seqₛ {y X Y : M} (h₀ : Exp.Seq₀ X Y) (hₛ : Exp.Seqₛ y X Y)
+lemma pow2_ext_of_seq₀_of_seqₛ {y X Y : M} (h₀ : Exponential.Seq₀ X Y) (hₛ : Exponential.Seqₛ y X Y)
     {i} (ne2 : i ≠ 2) (hi : i ≤ y^2) (ppi : PPow2 i) : Pow2 (ext i Y) := by
   induction i using order_induction_iSigmaZero
   · definability
@@ -213,12 +213,12 @@ lemma pow2_ext_of_seq₀_of_seqₛ {y X Y : M} (h₀ : Exp.Seq₀ X Y) (hₛ : E
       · have : ext i Y = 2*(ext (√i) Y)^2 := by simpa [ppi.sq_sqrt_eq ne2] using hodd.2
         simp [this, ppsq]
 
-lemma range_pow2 {x y : M} (h : Exp x y) : Pow2 y := by
+lemma range_pow2 {x y : M} (h : Exponential x y) : Pow2 y := by
   rcases h with (⟨rfl, rfl⟩ | ⟨X, bX, Y, bY, H₀, Hₛ, ⟨u, hu, ne2, ppu, rfl, rfl⟩⟩)
   · simp
   · exact pow2_ext_of_seq₀_of_seqₛ H₀ Hₛ ne2 hu ppu
 
-lemma le_sq_ext_of_seq₀_of_seqₛ {y X Y : M} (h₀ : Exp.Seq₀ X Y) (hₛ : Exp.Seqₛ y X Y)
+lemma le_sq_ext_of_seq₀_of_seqₛ {y X Y : M} (h₀ : Exponential.Seq₀ X Y) (hₛ : Exponential.Seqₛ y X Y)
     {i} (ne2 : i ≠ 2) (hi : i ≤ y^2) (ppi : PPow2 i) : i ≤ (ext i Y)^2 := by
   induction i using order_induction_iSigmaZero
   · definability
@@ -239,7 +239,7 @@ lemma le_sq_ext_of_seq₀_of_seqₛ {y X Y : M} (h₀ : Exp.Seq₀ X Y) (hₛ : 
 
 example {a b c : ℕ} : a * (b * c) = b * (a * c) := by exact Nat.mul_left_comm a b c
 
-lemma two_mul_ext_le_of_seq₀_of_seqₛ {y X Y : M} (h₀ : Exp.Seq₀ X Y) (hₛ : Exp.Seqₛ y X Y)
+lemma two_mul_ext_le_of_seq₀_of_seqₛ {y X Y : M} (h₀ : Exponential.Seq₀ X Y) (hₛ : Exponential.Seqₛ y X Y)
     {i} (ne2 : i ≠ 2) (hi : i ≤ y^2) (ppi : PPow2 i) : 2 * ext i Y ≤ i := by
   induction i using order_induction_iSigmaZero
   · definability
@@ -262,7 +262,7 @@ lemma two_mul_ext_le_of_seq₀_of_seqₛ {y X Y : M} (h₀ : Exp.Seq₀ X Y) (h�
           _           ≤ (√i)^2             := sq_le_sq.mpr IH
           _           = i                  := ppi.sq_sqrt_eq ne2
 
-lemma exp_exists_sq_of_exp_even {x y : M} : Exp (2 * x) y → ∃ y', y = y'^2 ∧ Exp x y' := by
+lemma exponential_exists_sq_of_exponential_even {x y : M} : Exponential (2 * x) y → ∃ y', y = y'^2 ∧ Exponential x y' := by
   rintro (⟨hx, rfl⟩ | ⟨X, _, Y, _, hseq₀, hseqₛ, i, hi, ne2, ppi, hXx, hYy⟩)
   · exact ⟨1, by simp [show x = 0 from by simpa using hx]⟩
   by_cases ne4 : i = 4
@@ -286,7 +286,7 @@ lemma exp_exists_sq_of_exp_even {x y : M} : Exp (2 * x) y → ∃ y', y = y'^2 �
       ⟨√i, sqrt_le_of_le_sq $ by simp [←hYy, hi], ppi.sqrt_ne_two ne2 ne4, ppi.sqrt ne2,
        by have : √i < i := sqrt_lt_self_of_one_lt ppi.one_lt
           simp [X', Y', this, ext_rem, ppi, ppi.sqrt ne2, hXx]⟩
-    have : Exp x (ext (√i) Y) :=
+    have : Exponential x (ext (√i) Y) :=
       Or.inr ⟨X', bX', Y', bY', hseq₀.rem ppi (ppi.four_lt ne2 ne4), hseqₛ', hseqₘ'⟩
     exact ⟨ext (√i) Y, hYy, this⟩
   · have : 2 ∣ ext i X := by simp [hXx]
@@ -295,7 +295,7 @@ lemma exp_exists_sq_of_exp_even {x y : M} : Exp (2 * x) y → ∃ y', y = y'^2 �
         ←mod_eq_zero_iff_dvd, one_lt_two]
     contradiction
 
-lemma bit_zero {x y : M} : Exp x y → Exp (2 * x) (y ^ 2) := by
+lemma bit_zero {x y : M} : Exponential x y → Exponential (2 * x) (y ^ 2) := by
   rintro (⟨hx, rfl⟩ | ⟨X, _, Y, _, hseq₀, hseqₛ, i, hi, ne2, ppi, hXx, hYy⟩)
   · rcases hx with rfl; simp
   have hxsqi : 2 * x < i ^ 2 := lt_of_lt_of_le (by simp [←hXx, ppi.pos]) (two_mul_le_sq ppi.two_le)
@@ -328,16 +328,16 @@ lemma bit_zero {x y : M} : Exp x y → Exp (2 * x) (y ^ 2) := by
      by simp at *; rw [ext_append_last, ext_append_last] <;> try simp [hxsqi, hysqi]⟩
   exact Or.inr <| ⟨X', bX', Y', bY', hseq₀', hseqₛ', hseqₘ'⟩
 
-lemma exp_even {x y : M} : Exp (2 * x) y ↔ ∃ y', y = y'^2 ∧ Exp x y' :=
-  ⟨exp_exists_sq_of_exp_even, by rintro ⟨y, rfl, h⟩; exact bit_zero h⟩
+lemma exponential_even {x y : M} : Exponential (2 * x) y ↔ ∃ y', y = y'^2 ∧ Exponential x y' :=
+  ⟨exponential_exists_sq_of_exponential_even, by rintro ⟨y, rfl, h⟩; exact bit_zero h⟩
 
-lemma exp_even_sq {x y : M} : Exp (2 * x) (y ^ 2) ↔ Exp x y :=
+lemma exponential_even_sq {x y : M} : Exponential (2 * x) (y ^ 2) ↔ Exponential x y :=
   ⟨by intro h
-      rcases exp_exists_sq_of_exp_even h with ⟨y', e, h⟩
+      rcases exponential_exists_sq_of_exponential_even h with ⟨y', e, h⟩
       simpa [show y = y' from by simpa using e] using h,
    bit_zero⟩
 
-lemma exp_exists_sq_of_exp_odd {x y : M} : Exp (2 * x + 1) y → ∃ y', y = 2 * y'^2 ∧ Exp x y' := by
+lemma exponential_exists_sq_of_exponential_odd {x y : M} : Exponential (2 * x + 1) y → ∃ y', y = 2 * y'^2 ∧ Exponential x y' := by
   rintro (⟨hx, rfl⟩ | ⟨X, _, Y, _, hseq₀, hseqₛ, i, hi, ne2, ppi, hXx, hYy⟩)
   · simp at hx
   by_cases ne4 : i = 4
@@ -367,11 +367,11 @@ lemma exp_exists_sq_of_exp_odd {x y : M} : Exp (2 * x + 1) y → ∃ y', y = 2 *
       ⟨√i, bsqi, ppi.sqrt_ne_two ne2 ne4, ppi.sqrt ne2,
        by have : √i < i := sqrt_lt_self_of_one_lt ppi.one_lt
           simp [X', Y', this, ext_rem, ppi, ppi.sqrt ne2, hXx]⟩
-    have : Exp x (ext (√i) Y) :=
+    have : Exponential x (ext (√i) Y) :=
       Or.inr ⟨X', bX', Y', bY', hseq₀.rem ppi (ppi.four_lt ne2 ne4), hseqₛ', hseqₘ'⟩
     exact ⟨ext (√i) Y, hYy, this⟩
 
-lemma bit_one {x y : M} : Exp x y → Exp (2 * x + 1) (2 * y ^ 2) := by
+lemma bit_one {x y : M} : Exponential x y → Exponential (2 * x + 1) (2 * y ^ 2) := by
   rintro (⟨hx, rfl⟩ | ⟨X, _, Y, _, hseq₀, hseqₛ, i, hi, ne2, ppi, hXx, hYy⟩)
   · rcases hx with rfl; simp
   have hxsqi : 2 * x + 1 < i ^ 2 := calc
@@ -412,16 +412,16 @@ lemma bit_one {x y : M} : Exp x y → Exp (2 * x + 1) (2 * y ^ 2) := by
      by simp [X', Y']; rw [ext_append_last, ext_append_last] <;> try simp [hxsqi, hysqi]⟩
   exact Or.inr <| ⟨X', bX', Y', bY', hseq₀', hseqₛ', hseqₘ'⟩
 
-lemma exp_odd {x y : M} : Exp (2 * x + 1) y ↔ ∃ y', y = 2 * y' ^ 2 ∧ Exp x y' :=
-  ⟨exp_exists_sq_of_exp_odd, by rintro ⟨y, rfl, h⟩; exact bit_one h⟩
+lemma exponential_odd {x y : M} : Exponential (2 * x + 1) y ↔ ∃ y', y = 2 * y' ^ 2 ∧ Exponential x y' :=
+  ⟨exponential_exists_sq_of_exponential_odd, by rintro ⟨y, rfl, h⟩; exact bit_one h⟩
 
-lemma exp_odd_two_mul_sq {x y : M} : Exp (2 * x + 1) (2 * y ^ 2) ↔ Exp x y :=
+lemma exponential_odd_two_mul_sq {x y : M} : Exponential (2 * x + 1) (2 * y ^ 2) ↔ Exponential x y :=
   ⟨by intro h
-      rcases exp_exists_sq_of_exp_odd h with ⟨y', e, h⟩
+      rcases exponential_exists_sq_of_exponential_odd h with ⟨y', e, h⟩
       simpa [show y = y' from by simpa using e] using h,
    bit_one⟩
 
-lemma two_le_ext_of_seq₀_of_seqₛ {y X Y : M} (h₀ : Exp.Seq₀ X Y) (hₛ : Exp.Seqₛ y X Y)
+lemma two_le_ext_of_seq₀_of_seqₛ {y X Y : M} (h₀ : Exponential.Seq₀ X Y) (hₛ : Exponential.Seqₛ y X Y)
     {i} (ne2 : i ≠ 2) (hi : i ≤ y^2) (ppi : PPow2 i) : 2 ≤ ext i Y := by
   induction i using order_induction_iSigmaZero
   · definability
@@ -442,7 +442,7 @@ lemma two_le_ext_of_seq₀_of_seqₛ {y X Y : M} (h₀ : Exp.Seq₀ X Y) (hₛ :
           _ ≤ 2 * (ext (√i) Y)^2 := by simp
           _ = ext i Y            := by simpa [ppi.sq_sqrt_eq ne2] using Eq.symm hodd.2
 
-lemma ext_le_ext_of_seq₀_of_seqₛ {y X Y : M} (h₀ : Exp.Seq₀ X Y) (hₛ : Exp.Seqₛ y X Y)
+lemma ext_le_ext_of_seq₀_of_seqₛ {y X Y : M} (h₀ : Exponential.Seq₀ X Y) (hₛ : Exponential.Seqₛ y X Y)
     {i} (ne2 : i ≠ 2) (hi : i ≤ y^2) (ppi : PPow2 i) : ext i X < ext i Y := by
   induction i using order_induction_iSigmaZero
   · definability
@@ -466,18 +466,18 @@ lemma ext_le_ext_of_seq₀_of_seqₛ {y X Y : M} (h₀ : Exp.Seq₀ X Y) (hₛ :
                   simp [one_add_one_eq_two]; exact (two_le_ext_of_seq₀_of_seqₛ h₀ hₛ (ppi.sqrt_ne_two ne2 ne4) (le_trans (by simp) hi) (ppi.sqrt ne2))))
           _       = ext i Y            := by simpa [ppi.sq_sqrt_eq ne2] using Eq.symm hodd.2
 
-lemma range_pos {x y : M} (h : Exp x y) : 0 < y := by
+lemma range_pos {x y : M} (h : Exponential x y) : 0 < y := by
   rcases h with (⟨rfl, rfl⟩ | ⟨X, bX, Y, bY, H₀, Hₛ, ⟨u, hu, ne2, ppu, rfl, rfl⟩⟩)
   · simp
   · have : 2 ≤ ext u Y := two_le_ext_of_seq₀_of_seqₛ H₀ Hₛ ne2 hu ppu
     exact lt_of_lt_of_le (by simp) this
 
-lemma dom_lt_range {x y : M} (h : Exp x y) : x < y := by
+lemma dom_lt_range {x y : M} (h : Exponential x y) : x < y := by
   rcases h with (⟨rfl, rfl⟩ | ⟨X, bX, Y, bY, H₀, Hₛ, ⟨u, hu, ne2, ppu, rfl, rfl⟩⟩)
   · simp
   · exact ext_le_ext_of_seq₀_of_seqₛ H₀ Hₛ ne2 hu ppu
 
-lemma not_exp_of_le {x y : M} (h : x ≤ y) : ¬Exp y x := by
+lemma not_exponential_of_le {x y : M} (h : x ≤ y) : ¬Exponential y x := by
   intro hxy; exact not_le.mpr (dom_lt_range hxy) h
 
 @[simp] lemma one_not_even (a : M) : 1 ≠ 2 * a := by
@@ -486,18 +486,18 @@ lemma not_exp_of_le {x y : M} (h : x ≤ y) : ¬Exp y x := by
   have : ¬(2 : M) ∣ 1 := not_dvd_of_lt (by simp) one_lt_two
   contradiction
 
-@[simp] lemma exp_two_four : Exp (2 : M) 4 := by
-  simpa [two_pow_two_eq_four] using (show Exp (1 : M) 2 from by simp).bit_zero
+@[simp] lemma exponential_two_four : Exponential (2 : M) 4 := by
+  simpa [two_pow_two_eq_four] using (show Exponential (1 : M) 2 from by simp).bit_zero
 
-lemma exp_succ {x y : M} : Exp (x + 1) y ↔ ∃ z, y = 2 * z ∧ Exp x z := by
-  suffices x < y → (Exp (x + 1) y ↔ ∃ z ≤ y, y = 2 * z ∧ Exp x z) by
+lemma exponential_succ {x y : M} : Exponential (x + 1) y ↔ ∃ z, y = 2 * z ∧ Exponential x z := by
+  suffices x < y → (Exponential (x + 1) y ↔ ∃ z ≤ y, y = 2 * z ∧ Exponential x z) by
     by_cases hxy : x < y
     · simp [this hxy]
       exact ⟨by rintro ⟨z, _, rfl, hz⟩; exact ⟨z, rfl, hz⟩,
              by rintro ⟨z, rfl, hz⟩; exact ⟨z, by simpa using hz⟩⟩
-    · simp [not_exp_of_le (show y ≤ x + 1 from le_add_right (by simpa using hxy))]
+    · simp [not_exponential_of_le (show y ≤ x + 1 from le_add_right (by simpa using hxy))]
       rintro z rfl
-      exact not_exp_of_le (le_trans le_two_mul_left $  by simpa using hxy)
+      exact not_exponential_of_le (le_trans le_two_mul_left $  by simpa using hxy)
   · revert x
     induction y using order_induction_iSigmaZero
     · definability
@@ -506,42 +506,42 @@ lemma exp_succ {x y : M} : Exp (x + 1) y ↔ ∃ z, y = 2 * z ∧ Exp x z := by
       rcases even_or_odd x with ⟨x, (rfl | rfl)⟩
       · constructor
         · intro H
-          rcases exp_odd.mp H with ⟨y, rfl, H'⟩
+          rcases exponential_odd.mp H with ⟨y, rfl, H'⟩
           exact ⟨y^2, by simp, rfl, H'.bit_zero⟩
         · rintro ⟨y, hy, rfl, H⟩
-          rcases exp_even.mp H with ⟨y, rfl, H'⟩
+          rcases exponential_even.mp H with ⟨y, rfl, H'⟩
           exact H'.bit_one
       · constructor
         · intro H
-          have : Exp (2 * (x + 1)) y := by simpa [mul_add, add_assoc, one_add_one_eq_two] using H
-          rcases exp_even.mp this with ⟨y, rfl, H'⟩
+          have : Exponential (2 * (x + 1)) y := by simpa [mul_add, add_assoc, one_add_one_eq_two] using H
+          rcases exponential_even.mp this with ⟨y, rfl, H'⟩
           have : 1 < y := by
             simpa using (show 1 < y^2 from lt_of_le_of_lt (by simp) hxy)
-          have : Exp (x + 1) y ↔ ∃ z ≤ y, y = 2 * z ∧ Exp x z :=
+          have : Exponential (x + 1) y ↔ ∃ z ≤ y, y = 2 * z ∧ Exponential x z :=
             IH y (lt_square_of_lt $ this) (lt_trans _ _ _ (by simp) H'.dom_lt_range)
           rcases this.mp H' with ⟨y, _, rfl, H''⟩
           exact ⟨2 * y ^ 2, by simp [sq, mul_assoc, mul_left_comm y 2],
             by simp [sq, mul_assoc, mul_left_comm y 2], H''.bit_one⟩
         · rintro ⟨y, _, rfl, H⟩
-          rcases exp_odd.mp H with ⟨y, rfl, H'⟩
+          rcases exponential_odd.mp H with ⟨y, rfl, H'⟩
           by_cases ne1 : y = 1
           · rcases ne1 with rfl
             rcases (show x = 0 from by simpa using H'.dom_lt_range)
             simp [one_add_one_eq_two, two_mul_two_eq_four]
           have : y < y^2 := lt_square_of_lt $ one_lt_iff_two_le.mpr $ H'.range_pow2.two_le ne1
-          have : Exp (x + 1) (2 * y) ↔ ∃ z ≤ 2 * y, 2 * y = 2 * z ∧ Exp x z :=
+          have : Exponential (x + 1) (2 * y) ↔ ∃ z ≤ 2 * y, 2 * y = 2 * z ∧ Exponential x z :=
             IH (2 * y) (by simp; exact lt_of_lt_of_le this le_two_mul_left)
               (lt_of_lt_of_le H'.dom_lt_range $ by simp)
-          have : Exp (x + 1) (2 * y) := this.mpr ⟨y, by simp, rfl, H'⟩
+          have : Exponential (x + 1) (2 * y) := this.mpr ⟨y, by simp, rfl, H'⟩
           simpa [sq, mul_add, add_assoc, mul_assoc, one_add_one_eq_two, mul_left_comm y 2] using this.bit_zero
 
-lemma exp_succ_mul_two {x y : M} : Exp (x + 1) (2 * y) ↔ Exp x y :=
-  ⟨by intro h; rcases exp_succ.mp h with ⟨y', e, h⟩; simpa [show y = y' from by simpa using e] using h,
-   by intro h; exact exp_succ.mpr ⟨y, rfl, h⟩⟩
+lemma exponential_succ_mul_two {x y : M} : Exponential (x + 1) (2 * y) ↔ Exponential x y :=
+  ⟨by intro h; rcases exponential_succ.mp h with ⟨y', e, h⟩; simpa [show y = y' from by simpa using e] using h,
+   by intro h; exact exponential_succ.mpr ⟨y, rfl, h⟩⟩
 
-alias ⟨of_succ_two_mul, succ⟩ := exp_succ_mul_two
+alias ⟨of_succ_two_mul, succ⟩ := exponential_succ_mul_two
 
-lemma one_le_ext_of_seq₀_of_seqₛ {y X Y : M} (h₀ : Exp.Seq₀ X Y) (hₛ : Exp.Seqₛ y X Y)
+lemma one_le_ext_of_seq₀_of_seqₛ {y X Y : M} (h₀ : Exponential.Seq₀ X Y) (hₛ : Exponential.Seqₛ y X Y)
     {i} (ne2 : i ≠ 2) (hi : i ≤ y^2) (ppi : PPow2 i) : 1 ≤ ext i X := by
   induction i using order_induction_iSigmaZero
   · definability
@@ -557,26 +557,26 @@ lemma one_le_ext_of_seq₀_of_seqₛ {y X Y : M} (h₀ : Exp.Seq₀ X Y) (hₛ :
       · have : ext i X = 2 * ext (√i) X + 1 := by simpa [ppi.sq_sqrt_eq ne2] using hodd.1
         simp [this]
 
-lemma zero_uniq {y : M} (h : Exp 0 y) : y = 1 := by
+lemma zero_uniq {y : M} (h : Exponential 0 y) : y = 1 := by
   rcases h with (⟨_, rfl⟩ | ⟨X, _, Y, _, H₀, Hₛ, ⟨u, hu, ne2, ppu, hX, _⟩⟩)
   · rfl
   · have : 1 ≤ ext u X  := one_le_ext_of_seq₀_of_seqₛ H₀ Hₛ ne2 hu ppu
     simp [hX] at this
 
-@[simp] lemma zero_uniq_iff {y : M} : Exp 0 y ↔ y = 1 :=
+@[simp] lemma zero_uniq_iff {y : M} : Exponential 0 y ↔ y = 1 :=
   ⟨zero_uniq, by rintro rfl; simp⟩
 
-lemma succ_lt_s {y : M} (h : Exp (x + 1) y) : 2 ≤ y := by
+lemma succ_lt_s {y : M} (h : Exponential (x + 1) y) : 2 ≤ y := by
   rcases h with (⟨h, rfl⟩ | ⟨X, _, Y, _, H₀, Hₛ, ⟨u, hu, ne2, ppu, _, hY⟩⟩)
   · simp at h
   · simpa [hY] using two_le_ext_of_seq₀_of_seqₛ H₀ Hₛ ne2 hu ppu
 
-protected lemma uniq {x y₁ y₂ : M} : Exp x y₁ → Exp x y₂ → y₁ = y₂ := by
+protected lemma uniq {x y₁ y₂ : M} : Exponential x y₁ → Exponential x y₂ → y₁ = y₂ := by
   intro h₁ h₂
   wlog h : y₁ ≤ y₂
   · exact Eq.symm <| this h₂ h₁ (show y₂ ≤ y₁ from le_of_not_ge h)
   revert x h y₁
-  suffices ∀ x < y₂, ∀ y₁ ≤ y₂, Exp x y₁ → Exp x y₂ → y₁ = y₂ by
+  suffices ∀ x < y₂, ∀ y₁ ≤ y₂, Exponential x y₁ → Exponential x y₂ → y₁ = y₂ by
     intro x y₁ h₁ h₂ hy; exact this x h₂.dom_lt_range y₁ hy h₁ h₂
   induction y₂ using order_induction_iSigmaZero
   · definability
@@ -584,16 +584,16 @@ protected lemma uniq {x y₁ y₂ : M} : Exp x y₁ → Exp x y₂ → y₁ = y�
     intro x _ y₁ h h₁ h₂
     rcases zero_or_succ x with (rfl | ⟨x, rfl⟩)
     · simp [h₁.zero_uniq, h₂.zero_uniq]
-    · rcases exp_succ.mp h₁ with ⟨y₁, rfl, h₁'⟩
-      rcases exp_succ.mp h₂ with ⟨y₂, rfl, h₂'⟩
+    · rcases exponential_succ.mp h₁ with ⟨y₁, rfl, h₁'⟩
+      rcases exponential_succ.mp h₂ with ⟨y₂, rfl, h₂'⟩
       have : y₁ = y₂ := IH y₂ (lt_mul_of_pos_of_one_lt_left h₂'.range_pos one_lt_two)
         x h₂'.dom_lt_range y₁ (by simpa using h) h₁' h₂'
       simp [this]
 
-protected lemma inj {x₁ x₂ y : M} : Exp x₁ y → Exp x₂ y → x₁ = x₂ := by
+protected lemma inj {x₁ x₂ y : M} : Exponential x₁ y → Exponential x₂ y → x₁ = x₂ := by
   intro h₁ h₂
   revert x₁ x₂ h₁ h₂
-  suffices ∀ x₁ < y, ∀ x₂ < y, Exp x₁ y → Exp x₂ y → x₁ = x₂ by
+  suffices ∀ x₁ < y, ∀ x₂ < y, Exponential x₁ y → Exponential x₂ y → x₁ = x₂ by
     intro x₁ x₂ h₁ h₂; exact this x₁ h₁.dom_lt_range x₂ h₂.dom_lt_range h₁ h₂
   induction y using order_induction_iSigmaZero
   · definability
@@ -602,30 +602,30 @@ protected lemma inj {x₁ x₂ y : M} : Exp x₁ y → Exp x₂ y → x₁ = x�
     rcases zero_or_succ x₁ with (rfl | ⟨x₁, rfl⟩) <;> rcases zero_or_succ x₂ with (rfl | ⟨x₂, rfl⟩)
     · rfl
     · rcases h₁.zero_uniq
-      rcases exp_succ.mp h₂ with ⟨z, hz⟩
+      rcases exponential_succ.mp h₂ with ⟨z, hz⟩
       simp at hz
     · rcases h₂.zero_uniq
-      rcases exp_succ.mp h₁ with ⟨z, hz⟩
+      rcases exponential_succ.mp h₁ with ⟨z, hz⟩
       simp at hz
-    · rcases exp_succ.mp h₁ with ⟨y, rfl, hy₁⟩
-      have hy₂ : Exp x₂ y := h₂.of_succ_two_mul
+    · rcases exponential_succ.mp h₁ with ⟨y, rfl, hy₁⟩
+      have hy₂ : Exponential x₂ y := h₂.of_succ_two_mul
       have : x₁ = x₂ :=
         IH y (lt_mul_of_pos_of_one_lt_left hy₁.range_pos one_lt_two)
           x₁ hy₁.dom_lt_range x₂ hy₂.dom_lt_range hy₁ hy₂
       simp [this]
 
-lemma exp_elim {x y : M} : Exp x y ↔ (x = 0 ∧ y = 1) ∨ ∃ x', ∃ y', x = x' + 1 ∧ y = 2 * y' ∧ Exp x' y' :=
+lemma exponential_elim {x y : M} : Exponential x y ↔ (x = 0 ∧ y = 1) ∨ ∃ x', ∃ y', x = x' + 1 ∧ y = 2 * y' ∧ Exponential x' y' :=
   ⟨by intro h
       rcases zero_or_succ x with (rfl | ⟨x', rfl⟩)
       · simp [h.zero_uniq]
-      · right; rcases exp_succ.mp h with ⟨y', rfl, H⟩
+      · right; rcases exponential_succ.mp h with ⟨y', rfl, H⟩
         exact ⟨x', y', rfl, rfl, H⟩,
    by rintro (⟨rfl, rfl⟩ | ⟨x, y, rfl, rfl, h⟩)
       · simp
       · exact h.succ⟩
 
-lemma monotone {x₁ x₂ y₁ y₂ : M} : Exp x₁ y₁ → Exp x₂ y₂ → x₁ < x₂ → y₁ < y₂ := by
-  suffices ∀ x₁ < y₁, ∀ y₂ ≤ y₁, ∀ x₂ < y₂, Exp x₁ y₁ → Exp x₂ y₂ → x₂ ≤ x₁ by
+lemma monotone {x₁ x₂ y₁ y₂ : M} : Exponential x₁ y₁ → Exponential x₂ y₂ → x₁ < x₂ → y₁ < y₂ := by
+  suffices ∀ x₁ < y₁, ∀ y₂ ≤ y₁, ∀ x₂ < y₂, Exponential x₁ y₁ → Exponential x₂ y₂ → x₂ ≤ x₁ by
     intro h₁ h₂; contrapose; simp
     intro hy
     exact this x₁ h₁.dom_lt_range y₂ hy x₂ h₂.dom_lt_range h₁ h₂
@@ -640,32 +640,32 @@ lemma monotone {x₁ x₂ y₁ y₂ : M} : Exp x₁ y₁ → Exp x₂ y₂ → x
       · have := h₂.range_pos; simp at this
       · exact False.elim <| not_lt.mpr h₂.succ_lt_s one_lt_two
     · simp
-    · rcases exp_succ.mp h₁ with ⟨y₁, rfl, h₁'⟩
-      rcases exp_succ.mp h₂ with ⟨y₂, rfl, h₂'⟩
+    · rcases exponential_succ.mp h₁ with ⟨y₁, rfl, h₁'⟩
+      rcases exponential_succ.mp h₂ with ⟨y₂, rfl, h₂'⟩
       have : x₂ ≤ x₁ := IH y₁ (lt_mul_of_pos_of_one_lt_left h₁'.range_pos one_lt_two)
         x₁ h₁'.dom_lt_range y₂ (le_of_mul_le_mul_left hy (by simp)) x₂ h₂'.dom_lt_range h₁' h₂'
       simpa using this
 
-lemma monotone_le {x₁ x₂ y₁ y₂ : M} (h₁ : Exp x₁ y₁) (h₂ : Exp x₂ y₂) : x₁ ≤ x₂ → y₁ ≤ y₂ := by
+lemma monotone_le {x₁ x₂ y₁ y₂ : M} (h₁ : Exponential x₁ y₁) (h₂ : Exponential x₂ y₂) : x₁ ≤ x₂ → y₁ ≤ y₂ := by
   rintro (rfl | h)
   · exact (h₁.uniq h₂).le
   · exact le_of_lt (monotone h₁ h₂ h)
 
-lemma monotone_iff {x₁ x₂ y₁ y₂ : M} (h₁ : Exp x₁ y₁) (h₂ : Exp x₂ y₂) : x₁ < x₂ ↔ y₁ < y₂ := by
+lemma monotone_iff {x₁ x₂ y₁ y₂ : M} (h₁ : Exponential x₁ y₁) (h₂ : Exponential x₂ y₂) : x₁ < x₂ ↔ y₁ < y₂ := by
   constructor
   · exact monotone h₁ h₂
   · contrapose; simp; exact monotone_le h₂ h₁
 
-lemma monotone_le_iff {x₁ x₂ y₁ y₂ : M} (h₁ : Exp x₁ y₁) (h₂ : Exp x₂ y₂) : x₁ ≤ x₂ ↔ y₁ ≤ y₂ := by
+lemma monotone_le_iff {x₁ x₂ y₁ y₂ : M} (h₁ : Exponential x₁ y₁) (h₂ : Exponential x₂ y₂) : x₁ ≤ x₂ ↔ y₁ ≤ y₂ := by
   constructor
   · exact monotone_le h₁ h₂
   · contrapose; simp; exact monotone h₂ h₁
 
-lemma add_mul {x₁ x₂ y₁ y₂ : M} (h₁ : Exp x₁ y₁) (h₂ : Exp x₂ y₂) : Exp (x₁ + x₂) (y₁ * y₂) := by
+lemma add_mul {x₁ x₂ y₁ y₂ : M} (h₁ : Exponential x₁ y₁) (h₂ : Exponential x₂ y₂) : Exponential (x₁ + x₂) (y₁ * y₂) := by
   wlog hy : y₁ ≥ y₂
   · simpa [add_comm, mul_comm] using this h₂ h₁ (le_of_not_ge hy)
   revert y₂
-  suffices ∀ y₂ ≤ y₁, Exp x₂ y₂ → Exp (x₁ + x₂) (y₁ * y₂) by
+  suffices ∀ y₂ ≤ y₁, Exponential x₂ y₂ → Exponential (x₁ + x₂) (y₁ * y₂) by
     intro y₂ h₂ hy; exact this y₂ hy h₂
   induction x₂ using induction_iSigmaZero
   · definability
@@ -674,11 +674,11 @@ lemma add_mul {x₁ x₂ y₁ y₂ : M} (h₁ : Exp x₁ y₁) (h₂ : Exp x₂ 
     simpa [show y₂ = 1 from h₂.zero_uniq] using h₁
   case succ x₂ IH =>
     intro y₂ hy h₂
-    rcases exp_succ.mp h₂ with ⟨y₂, rfl, H₂⟩
-    have : Exp (x₁ + x₂) (y₁ * y₂) := IH y₂ (le_trans (by simp) hy) H₂
+    rcases exponential_succ.mp h₂ with ⟨y₂, rfl, H₂⟩
+    have : Exponential (x₁ + x₂) (y₁ * y₂) := IH y₂ (le_trans (by simp) hy) H₂
     simpa [←add_assoc, mul_left_comm y₁ 2 y₂] using this.succ
 
-end Exp
+end Exponential
 
 end ISigma₀
 
@@ -686,9 +686,9 @@ section ISigma₁
 
 variable [M ⊧ₘ* 𝐈𝚺₁]
 
-namespace Exp
+namespace Exponential
 
-lemma range_exists (x : M) : ∃ y, Exp x y := by
+lemma range_exists (x : M) : ∃ y, Exponential x y := by
   induction x using induction_iSigmaOne
   · definability
   case zero => exact ⟨1, by simp⟩
@@ -696,41 +696,41 @@ lemma range_exists (x : M) : ∃ y, Exp x y := by
     rcases IH with ⟨y, IH⟩
     exact ⟨2 * y, IH.succ⟩
 
-lemma range_exists_unique (x : M) : ∃! y, Exp x y := by
+lemma range_exists_unique (x : M) : ∃! y, Exponential x y := by
   rcases range_exists x with ⟨y, h⟩
   exact ExistsUnique.intro y h (by intro y' h'; exact h'.uniq h)
 
-end Exp
+end Exponential
 
-instance : _root_.Exp M := ⟨fun a ↦ Classical.choose! (Exp.range_exists_unique a)⟩
+instance : _root_.Exp M := ⟨fun a ↦ Classical.choose! (Exponential.range_exists_unique a)⟩
 
 section exponential
 
-lemma exp_exponential (a : M) : Exp a (exp a) := Classical.choose!_spec (Exp.range_exists_unique a)
+lemma exp_exponential (a : M) : Exponential a (exp a) := Classical.choose!_spec (Exponential.range_exists_unique a)
 
-lemma exponential_graph {a b : M} : a = exp b ↔ Exp b a := Classical.choose!_eq_iff _
+lemma exponential_graph {a b : M} : a = exp b ↔ Exponential b a := Classical.choose!_eq_iff _
 
-def expDef : Δ₀-Sentence 2 := ⟨“!Exp.def [#1, #0]”, by simp⟩
+def expDef : Δ₀-Sentence 2 := ⟨“!Exponential.def [#1, #0]”, by simp⟩
 
 -- #eval expDef.val
 
-lemma exp_defined : Δ₀-Function₁ (Exp.exp : M → M) via expDef := by
-  intro v; simp [expDef, exponential_graph, Exp.defined.pval]
+lemma exp_defined_deltaZero : Δ₀-Function₁ (Exp.exp : M → M) via expDef := by
+  intro v; simp [expDef, exponential_graph, Exponential.defined.pval]
 
-instance exponential_definable : DefinableFunction₁ ℒₒᵣ Σ 0 (Exp.exp : M → M) := defined_to_with_param _ exp_defined
+instance exp_definable_deltaZero : DefinableFunction₁ ℒₒᵣ Σ 0 (Exp.exp : M → M) := defined_to_with_param _ exp_defined_deltaZero
 
-lemma exponential_of_exp {a b : M} (h : Exp a b) : exp a = b :=
+lemma exp_of_exponential {a b : M} (h : Exponential a b) : exp a = b :=
   Eq.symm <| exponential_graph.mpr h
 
-lemma exponential_inj : Function.Injective (Exp.exp : M → M) := λ a _ H ↦
+lemma exp_inj : Function.Injective (Exp.exp : M → M) := λ a _ H ↦
   (exp_exponential a).inj (exponential_graph.mp H)
 
-@[simp] lemma exp_zero : exp (0 : M) = 1 := exponential_of_exp (by simp)
+@[simp] lemma exp_zero : exp (0 : M) = 1 := exp_of_exponential (by simp)
 
-@[simp] lemma exp_one : exp (1 : M) = 2 := exponential_of_exp (by simp)
+@[simp] lemma exp_one : exp (1 : M) = 2 := exp_of_exponential (by simp)
 
 lemma exp_succ (a : M) : exp (a + 1) = 2 * exp a :=
-  exponential_of_exp <| Exp.exp_succ_mul_two.mpr <| exp_exponential a
+  exp_of_exponential <| Exponential.exponential_succ_mul_two.mpr <| exp_exponential a
 
 @[simp] lemma numeral_two_eq_two : (ORingSymbol.numeral 2 : M) = 2 := by simp [numeral_eq_natCast]
 
@@ -742,7 +742,7 @@ instance models_exponential_of_models_iSigmaOne : M ⊧ₘ* 𝐄𝐗𝐏 :=
   ⟨by intro f hf; rcases hf <;> simp [models_iff, exp_succ]⟩
 
 lemma exp_even (a : M) : exp (2 * a) = (exp a)^2 :=
-  exponential_of_exp <| Exp.exp_even_sq.mpr <| exp_exponential a
+  exp_of_exponential <| Exponential.exponential_even_sq.mpr <| exp_exponential a
 
 @[simp] lemma lt_exp (a : M) : a < exp a := (exp_exponential a).dom_lt_range
 
@@ -752,11 +752,11 @@ lemma exp_even (a : M) : exp (2 * a) = (exp a)^2 :=
 
 @[simp] lemma exp_pow2 (a : M) : Pow2 (exp a) := (exp_exponential a).range_pow2
 
-@[simp] lemma exponential_monotone {a b : M} : exp a < exp b ↔ a < b :=
-  Iff.symm <| Exp.monotone_iff (exp_exponential a) (exp_exponential b)
+@[simp] lemma exp_monotone {a b : M} : exp a < exp b ↔ a < b :=
+  Iff.symm <| Exponential.monotone_iff (exp_exponential a) (exp_exponential b)
 
-@[simp] lemma exponential_monotone_le {a b : M} : exp a ≤ exp b ↔ a ≤ b :=
-  Iff.symm <| Exp.monotone_le_iff (exp_exponential a) (exp_exponential b)
+@[simp] lemma exp_monotone_le {a b : M} : exp a ≤ exp b ↔ a ≤ b :=
+  Iff.symm <| Exponential.monotone_le_iff (exp_exponential a) (exp_exponential b)
 
 end exponential
 
