Arithmetization/IDeltaZero/Exponential/Log.lean
@@ -14,21 +14,21 @@ section ISigma₀
 
 variable [M ⊧ₘ* 𝐈𝚫₀]
 
-lemma log_exists_unique_pos {y : M} (hy : 0 < y) : ∃! x, x < y ∧ ∃ y' ≤ y, Exp x y' ∧ y < 2 * y' := by
-  have : ∃ x < y, ∃ y' ≤ y, Exp x y' ∧ y < 2 * y' := by
+lemma log_exists_unique_pos {y : M} (hy : 0 < y) : ∃! x, x < y ∧ ∃ y' ≤ y, Exponential x y' ∧ y < 2 * y' := by
+  have : ∃ x < y, ∃ y' ≤ y, Exponential x y' ∧ y < 2 * y' := by
     induction y using hierarchy_polynomial_induction_oRing_sigma₀
     · definability
     case zero => simp at hy
     case even y _ IH =>
-      rcases (IH (by simpa using hy) : ∃ x < y, ∃ y' ≤ y, Exp x y' ∧ y < 2 * y') with ⟨x, hxy, y', gey, H, lty⟩
+      rcases (IH (by simpa using hy) : ∃ x < y, ∃ y' ≤ y, Exponential x y' ∧ y < 2 * y') with ⟨x, hxy, y', gey, H, lty⟩
       exact ⟨x + 1, lt_of_lt_of_le (by simp [hxy]) (succ_le_double_of_pos (pos_of_gt hxy)),
-        2 * y', by simpa using gey, Exp.exp_succ_mul_two.mpr H, by simpa using lty⟩
+        2 * y', by simpa using gey, Exponential.exponential_succ_mul_two.mpr H, by simpa using lty⟩
     case odd y IH =>
       rcases (zero_le y : 0 ≤ y) with (rfl | pos)
       · simp; exact ⟨1, by simp [one_lt_two]⟩
-      · rcases (IH pos : ∃ x < y, ∃ y' ≤ y, Exp x y' ∧ y < 2 * y') with ⟨x, hxy, y', gey, H, lty⟩
+      · rcases (IH pos : ∃ x < y, ∃ y' ≤ y, Exponential x y' ∧ y < 2 * y') with ⟨x, hxy, y', gey, H, lty⟩
         exact ⟨x + 1, by simp; exact lt_of_lt_of_le hxy (by simp),
-          2 * y', le_trans (by simpa using gey) le_self_add, Exp.exp_succ_mul_two.mpr H, two_mul_add_one_lt_two_mul_of_lt lty⟩
+          2 * y', le_trans (by simpa using gey) le_self_add, Exponential.exponential_succ_mul_two.mpr H, two_mul_add_one_lt_two_mul_of_lt lty⟩
   rcases this with ⟨x, hx⟩
   exact ExistsUnique.intro x hx (fun x' ↦ by
     intro hx'
@@ -37,14 +37,14 @@ lemma log_exists_unique_pos {y : M} (hy : 0 < y) : ∃! x, x < y ∧ ∃ y' ≤ 
     · exact this hy x' hx' x hx (Ne.symm A) (lt_of_le_of_ne (by simpa using lt) A)
     rcases hx with ⟨_, z, _, H, hyz⟩
     rcases hx' with ⟨_, z', hzy', H', _⟩
-    have : z < z' := Exp.monotone H H' lt
+    have : z < z' := Exponential.monotone H H' lt
     have : y < y := calc
       y < 2 * z := hyz
       _ ≤ z'    := (Pow2.lt_iff_two_mul_le H.range_pow2 H'.range_pow2).mp this
       _ ≤ y     := hzy'
     simp at this)
 
-lemma log_exists_unique (y : M) : ∃! x, (y = 0 → x = 0) ∧ (0 < y → x < y ∧ ∃ y' ≤ y, Exp x y' ∧ y < 2 * y') := by
+lemma log_exists_unique (y : M) : ∃! x, (y = 0 → x = 0) ∧ (0 < y → x < y ∧ ∃ y' ≤ y, Exponential x y' ∧ y < 2 * y') := by
   by_cases hy : y = 0
   · rcases hy; simp
   · simp [hy, pos_iff_ne_zero.mpr hy, log_exists_unique_pos]
@@ -54,7 +54,7 @@ def log (a : M) : M := Classical.choose! (log_exists_unique a)
 @[simp] lemma log_zero : log (0 : M) = 0 :=
   (Classical.choose!_spec (log_exists_unique (0 : M))).1 rfl
 
-lemma log_pos {y : M} (pos : 0 < y) : ∃ y' ≤ y, Exp (log y) y' ∧ y < 2 * y' :=
+lemma log_pos {y : M} (pos : 0 < y) : ∃ y' ≤ y, Exponential (log y) y' ∧ y < 2 * y' :=
   ((Classical.choose!_spec (log_exists_unique y)).2 pos).2
 
 lemma log_lt_self_of_pos {y : M} (pos : 0 < y) : log y < y :=
@@ -65,18 +65,18 @@ lemma log_lt_self_of_pos {y : M} (pos : 0 < y) : log y < y :=
   · simp
   · exact le_of_lt <| log_lt_self_of_pos pos
 
-lemma log_graph {x y : M} : x = log y ↔ (y = 0 → x = 0) ∧ (0 < y → x < y ∧ ∃ y' ≤ y, Exp x y' ∧ y < 2 * y') := Classical.choose!_eq_iff _
+lemma log_graph {x y : M} : x = log y ↔ (y = 0 → x = 0) ∧ (0 < y → x < y ∧ ∃ y' ≤ y, Exponential x y' ∧ y < 2 * y') := Classical.choose!_eq_iff _
 
-def logDef : Δ₀-Sentence 2 := ⟨“(#1 = 0 → #0 = 0) ∧ (0 < #1 → #0 < #1 ∧ ∃[#0 < #2 + 1] (!Exp.def [#1, #0] ∧ #2 < 2 * #0))”, by simp⟩
+def logDef : Δ₀-Sentence 2 := ⟨“(#1 = 0 → #0 = 0) ∧ (0 < #1 → #0 < #1 ∧ ∃[#0 < #2 + 1] (!Exponential.def [#1, #0] ∧ #2 < 2 * #0))”, by simp⟩
 
 lemma log_defined : Δ₀-Function₁ (log : M → M) via logDef := by
-  intro v; simp [logDef, log_graph, Exp.defined.pval, ←le_iff_lt_succ, numeral_eq_natCast]
+  intro v; simp [logDef, log_graph, Exponential.defined.pval, ←le_iff_lt_succ, numeral_eq_natCast]
 
 instance log_definable : DefinableFunction₁ ℒₒᵣ Σ 0 (log : M → M) := defined_to_with_param _ log_defined
 
 instance : PolyBounded₁ ℒₒᵣ (log : M → M) := ⟨#0, λ _ ↦ by simp⟩
 
-lemma log_eq_of_pos {x y : M} (pos : 0 < y) {y'} (H : Exp x y') (hy' : y' ≤ y) (hy : y < 2 * y') : log y = x :=
+lemma log_eq_of_pos {x y : M} (pos : 0 < y) {y'} (H : Exponential x y') (hy' : y' ≤ y) (hy : y < 2 * y') : log y = x :=
   (log_exists_unique_pos pos).unique ⟨log_lt_self_of_pos pos, log_pos pos⟩ ⟨lt_of_lt_of_le H.dom_lt_range hy', y', hy', H, hy⟩
 
 @[simp] lemma log_one : log (1 : M) = 0 := log_eq_of_pos (by simp) (y' := 1) (by simp) (by rfl) (by simp [one_lt_two])
@@ -85,17 +85,17 @@ lemma log_eq_of_pos {x y : M} (pos : 0 < y) {y'} (H : Exp x y') (hy' : y' ≤ y)
 
 lemma log_two_mul_of_pos {y : M} (pos : 0 < y) : log (2 * y) = log y + 1 := by
   rcases log_pos pos with ⟨y', hy', H, hy⟩
-  exact log_eq_of_pos (by simpa using pos) (Exp.exp_succ_mul_two.mpr H) (by simpa using hy') (by simpa using hy)
+  exact log_eq_of_pos (by simpa using pos) (Exponential.exponential_succ_mul_two.mpr H) (by simpa using hy') (by simpa using hy)
 
 lemma log_two_mul_add_one_of_pos {y : M} (pos : 0 < y) : log (2 * y + 1) = log y + 1 := by
   rcases log_pos pos with ⟨y', hy', H, hy⟩
-  exact log_eq_of_pos (by simp) (Exp.exp_succ_mul_two.mpr H)
+  exact log_eq_of_pos (by simp) (Exponential.exponential_succ_mul_two.mpr H)
     (le_trans (by simpa using hy') le_self_add) (two_mul_add_one_lt_two_mul_of_lt hy)
 
-lemma Exp.log_eq_of_exp {x y : M} (H : Exp x y) : log y = x :=
+lemma Exponential.log_eq_of_exp {x y : M} (H : Exponential x y) : log y = x :=
   log_eq_of_pos H.range_pos H (by { rfl }) (lt_mul_of_pos_of_one_lt_left H.range_pos one_lt_two)
 
-lemma exp_of_pow2 {p : M} (pp : Pow2 p) : Exp (log p) p := by
+lemma exponential_of_pow2 {p : M} (pp : Pow2 p) : Exponential (log p) p := by
   rcases log_pos pp.pos with ⟨q, hq, H, hp⟩
   suffices p = q by simpa [this] using H
   by_contra ne
@@ -109,8 +109,8 @@ lemma log_mul_pow2_add_of_lt {a p b : M} (pos : 0 < a) (pp : Pow2 p) (hb : b < p
   rcases log_pos pos with ⟨a', ha', Ha, ha⟩
   rcases log_pos pp.pos with ⟨p', hp', Hp, hp⟩
   exact log_eq_of_pos (lt_of_lt_of_le (mul_pos pos pp.pos) le_self_add)
-    (Exp.add_mul Ha Hp) (le_trans (mul_le_mul' ha' hp') le_self_add) (by
-      rcases Hp.uniq (exp_of_pow2 pp)
+    (Exponential.add_mul Ha Hp) (le_trans (mul_le_mul' ha' hp') le_self_add) (by
+      rcases Hp.uniq (exponential_of_pow2 pp)
       calc
         a * p + b < a * p + p    := by simp [hb]
         _         = (a + 1) * p  := by simp [add_mul]
@@ -127,7 +127,7 @@ lemma log_monotone {a b : M} (h : a ≤ b) : log a ≤ log b := by
   rcases log_pos posa with ⟨a', ha', Ha, _⟩
   rcases log_pos posb with ⟨b', _, Hb, hb⟩
   by_contra lt
-  have : b' < a' := (Exp.monotone_iff Hb Ha).mp (by simpa using lt)
+  have : b' < a' := (Exponential.monotone_iff Hb Ha).mp (by simpa using lt)
   have : b < b := calc
     b < 2 * b' := hb
     _ ≤ a'     := (Pow2.lt_iff_two_mul_le Hb.range_pow2 Ha.range_pow2).mp this
@@ -169,7 +169,7 @@ instance : PolyBounded₁ ℒₒᵣ (‖·‖ : M → M) := ⟨#0, λ _ ↦ by s
 
 @[simp] lemma length_one : ‖(1 : M)‖ = 1 := by simp [length_eq_binaryLength]
 
-lemma Exp.length_eq {x y : M} (H : Exp x y) : ‖y‖ = x + 1 := by
+lemma Exponential.length_eq {x y : M} (H : Exponential x y) : ‖y‖ = x + 1 := by
   simp [length_of_pos H.range_pos]; exact H.log_eq_of_exp
 
 lemma length_two_mul_of_pos {a : M} (pos : 0 < a) : ‖2 * a‖ = ‖a‖ + 1 := by
@@ -205,50 +205,50 @@ lemma le_log_of_lt_length {a b : M} (h : a < ‖b‖) : a ≤ log b := by
   have : 0 < b := pos_of_lt_length h
   exact le_iff_lt_succ.mpr (by simpa [length_of_pos this] using h)
 
-lemma exp_log_le_self {a b : M} (pos : 0 < a) (h : Exp (log a) b) : b ≤ a := by
+lemma exponential_log_le_self {a b : M} (pos : 0 < a) (h : Exponential (log a) b) : b ≤ a := by
   rcases log_pos pos with ⟨_, _, H, _⟩; rcases H.uniq h
   assumption
 
-lemma lt_exp_log_self {a b : M} (h : Exp (log a) b) : a < 2 * b := by
+lemma lt_exponential_log_self {a b : M} (h : Exponential (log a) b) : a < 2 * b := by
   rcases zero_le a with (rfl | pos)
   · simp at h; simp [h]
   rcases log_pos pos with ⟨_, _, H, _⟩; rcases H.uniq h
   assumption
 
-lemma lt_exp_len_self {a b : M} (h : Exp ‖a‖ b) : a < b := by
+lemma lt_exp_len_self {a b : M} (h : Exponential ‖a‖ b) : a < b := by
   rcases zero_le a with (rfl | pos)
   · simp at h; simp [h]
   simp [length_of_pos pos] at h
-  rcases Exp.exp_succ.mp h with ⟨b, rfl, H⟩
-  exact lt_exp_log_self H
+  rcases Exponential.exponential_succ.mp h with ⟨b, rfl, H⟩
+  exact lt_exponential_log_self H
 
-lemma le_iff_le_log_of_exp {x y a : M} (H : Exp x y) (pos : 0 < a) : y ≤ a ↔ x ≤ log a :=
+lemma le_iff_le_log_of_exp {x y a : M} (H : Exponential x y) (pos : 0 < a) : y ≤ a ↔ x ≤ log a :=
   ⟨by rcases H.log_eq_of_exp; exact log_monotone,
-   fun h ↦ by rcases log_pos pos with ⟨a', ha', Haa', _⟩; exact le_trans (Exp.monotone_le H Haa' h) ha'⟩
+   fun h ↦ by rcases log_pos pos with ⟨a', ha', Haa', _⟩; exact le_trans (Exponential.monotone_le H Haa' h) ha'⟩
 
-lemma le_iff_lt_length_of_exp {x y a : M} (H : Exp x y) : y ≤ a ↔ x < ‖a‖ := by
+lemma le_iff_lt_length_of_exp {x y a : M} (H : Exponential x y) : y ≤ a ↔ x < ‖a‖ := by
   rcases zero_le a with (rfl | pos)
   · simp; exact pos_iff_ne_zero.mp H.range_pos
   simp [le_iff_le_log_of_exp H pos, length_of_pos pos, ←le_iff_lt_succ]
 
-lemma Exp.lt_iff_log_lt {x y a : M} (H : Exp x y) (pos : 0 < a) : a < y ↔ log a < x :=
+lemma Exponential.lt_iff_log_lt {x y a : M} (H : Exponential x y) (pos : 0 < a) : a < y ↔ log a < x :=
   not_iff_not.mp (by simpa using le_iff_le_log_of_exp H pos)
 
-lemma Exp.lt_iff_len_le {x y a : M} (H : Exp x y) : a < y ↔ ‖a‖ ≤ x := not_iff_not.mp (by simpa using le_iff_lt_length_of_exp H)
+lemma Exponential.lt_iff_len_le {x y a : M} (H : Exponential x y) : a < y ↔ ‖a‖ ≤ x := not_iff_not.mp (by simpa using le_iff_lt_length_of_exp H)
 
-lemma Exp.le_of_lt_length {x y a : M} (H : Exp x y) : x < ‖a‖ → y ≤ a := fun h ↦
+lemma Exponential.le_of_lt_length {x y a : M} (H : Exponential x y) : x < ‖a‖ → y ≤ a := fun h ↦
   (le_iff_lt_length_of_exp H).mpr h
 
-lemma Exp.le_log {x y : M} (H : Exp x y) : x ≤ log y := (le_iff_le_log_of_exp H H.range_pos).mp (by rfl)
+lemma Exponential.le_log {x y : M} (H : Exponential x y) : x ≤ log y := (le_iff_le_log_of_exp H H.range_pos).mp (by rfl)
 
-lemma Exp.lt_length {x y : M} (H : Exp x y) : x < ‖y‖ := (le_iff_lt_length_of_exp H).mp (by rfl)
+lemma Exponential.lt_length {x y : M} (H : Exponential x y) : x < ‖y‖ := (le_iff_lt_length_of_exp H).mp (by rfl)
 
-lemma lt_exp_length {a b : M} (h : Exp ‖a‖ b) : a < b := by
+lemma lt_exponential_length {a b : M} (h : Exponential ‖a‖ b) : a < b := by
   rcases zero_le a with (rfl | pos)
   · simp at h; simp [h]
   simp [length_of_pos pos] at h
-  rcases Exp.exp_succ.mp h with ⟨b, rfl, H⟩
-  exact lt_exp_log_self H
+  rcases Exponential.exponential_succ.mp h with ⟨b, rfl, H⟩
+  exact lt_exponential_log_self H
 
 lemma sq_len_le_three_mul (a : M) : ‖a‖ ^ 2 ≤ 3 * a := by
   induction a using hierarchy_polynomial_induction_oRing_sigma₀
@@ -274,8 +274,8 @@ lemma sq_len_le_three_mul (a : M) : ‖a‖ ^ 2 ≤ 3 * a := by
       _               = 3 * (2 * a)           := by simp_all only [←two_add_one_eq_three, two_mul, add_mul, add_assoc, one_mul]
       _               ≤ 3 * (2 * a + 1)       := by simp
 
-lemma brange_exists_unique (a : M) : ∀ x < ‖a‖, ∃! y, Exp x y := by
-  suffices ∀ x < ‖a‖, ∃ y ≤ a, Exp x y by
+lemma brange_exists_unique (a : M) : ∀ x < ‖a‖, ∃! y, Exponential x y := by
+  suffices ∀ x < ‖a‖, ∃ y ≤ a, Exponential x y by
     intro x hx; rcases this x hx with ⟨_, _, H⟩
     exact ExistsUnique.intro _ H (fun y' H' ↦ H'.uniq H)
   intro x
@@ -287,12 +287,12 @@ lemma brange_exists_unique (a : M) : ∀ x < ‖a‖, ∃! y, Exp x y := by
     exact ⟨1, pos_iff_one_le.mp this, by simp⟩
   case succ x IH =>
     intro hx
-    rcases (IH (lt_of_le_of_lt (by simp) hx) : ∃ y ≤ a, Exp x y) with ⟨y, hy, H⟩
+    rcases (IH (lt_of_le_of_lt (by simp) hx) : ∃ y ≤ a, Exponential x y) with ⟨y, hy, H⟩
     have : 0 < a := by by_contra A; rcases (show a = 0 from by simpa using A); simp_all
     have : 2 * y ≤ a := (le_iff_le_log_of_exp H.succ this).mpr (le_log_of_lt_length hx)
     exact ⟨2 * y, this, H.succ⟩
 
-lemma bexp_exists_unique (a x : M) : ∃! y, (x < ‖a‖ → Exp x y) ∧ (‖a‖ ≤ x → y = 0) := by
+lemma bexp_exists_unique (a x : M) : ∃! y, (x < ‖a‖ → Exponential x y) ∧ (‖a‖ ≤ x → y = 0) := by
   by_cases hx : x < ‖a‖
   · simp [hx, show ¬‖a‖ ≤ x from by simpa using hx, log_exists_unique_pos]
     exact brange_exists_unique a x hx
@@ -301,7 +301,7 @@ lemma bexp_exists_unique (a x : M) : ∃! y, (x < ‖a‖ → Exp x y) ∧ (‖a
 /-- `bexp a x = exp x` if `x < ‖a‖`; `= 0` o.w.-/
 def bexp (a x : M) : M := Classical.choose! (bexp_exists_unique a x)
 
-lemma exp_bexp_of_lt {a x : M} (h : x < ‖a‖) : Exp x (bexp a x) :=
+lemma exp_bexp_of_lt {a x : M} (h : x < ‖a‖) : Exponential x (bexp a x) :=
   (Classical.choose!_spec (bexp_exists_unique a x)).1 h
 
 lemma bexp_eq_zero_of_le {a x : M} (h : ‖a‖ ≤ x) : bexp a x = 0 :=
@@ -309,7 +309,7 @@ lemma bexp_eq_zero_of_le {a x : M} (h : ‖a‖ ≤ x) : bexp a x = 0 :=
 
 @[simp] lemma bexp_zero (x : M): bexp 0 x = 0 := bexp_eq_zero_of_le (by simp)
 
-@[simp] lemma exp_bexp_of_lt_iff {a x : M} : Exp x (bexp a x) ↔ x < ‖a‖ :=
+@[simp] lemma exp_bexp_of_lt_iff {a x : M} : Exponential x (bexp a x) ↔ x < ‖a‖ :=
   ⟨by intro h; by_contra A
       have : bexp a x = 0 := bexp_eq_zero_of_le (not_lt.mp A)
       simp [this] at h
@@ -322,31 +322,31 @@ lemma bexp_eq_zero_of_le {a x : M} (h : ‖a‖ ≤ x) : bexp a x = 0 :=
     exact (le_iff_le_log_of_exp (exp_bexp_of_lt lt) this).mpr (le_log_of_lt_length lt)
   · simp [bexp_eq_zero_of_le le]
 
-lemma bexp_graph {y a x : M} : y = bexp a x ↔ ∃ l ≤ a, l = ‖a‖ ∧ (x < l → Exp x y) ∧ (l ≤ x → y = 0) :=
+lemma bexp_graph {y a x : M} : y = bexp a x ↔ ∃ l ≤ a, l = ‖a‖ ∧ (x < l → Exponential x y) ∧ (l ≤ x → y = 0) :=
   ⟨by rintro rfl; exact ⟨‖a‖, by simp, rfl, exp_bexp_of_lt, bexp_eq_zero_of_le⟩, by
     rintro ⟨_, _, rfl, hlt, hle⟩
     rcases show x < ‖a‖ ∨ ‖a‖ ≤ x from lt_or_ge _ _ with (lt | le)
     · exact (hlt lt).uniq (exp_bexp_of_lt lt)
     · rcases hle le; simp [bexp_eq_zero_of_le le]⟩
 
-def bexpDef : Δ₀-Sentence 3 := ⟨“∃[#0 < #2 + 1] (!lengthDef [#0, #2] ∧ (#3 < #0 → !Exp.def [#3, #1]) ∧ (#0 ≤ #3 → #1 = 0))”, by simp⟩
+def bexpDef : Δ₀-Sentence 3 := ⟨“∃[#0 < #2 + 1] (!lengthDef [#0, #2] ∧ (#3 < #0 → !Exponential.def [#3, #1]) ∧ (#0 ≤ #3 → #1 = 0))”, by simp⟩
 
 lemma bexp_defined : Δ₀-Function₂ (bexp : M → M → M) via bexpDef := by
-  intro v; simp [bexpDef, bexp_graph, Exp.defined.pval, length_defined.pval, ←le_iff_lt_succ]
+  intro v; simp [bexpDef, bexp_graph, Exponential.defined.pval, length_defined.pval, ←le_iff_lt_succ]
 
 instance bexp_definable : DefinableFunction₂ ℒₒᵣ Σ 0 (bexp : M → M → M) := defined_to_with_param _ bexp_defined
 
 instance : PolyBounded₂ ℒₒᵣ (bexp : M → M → M) := ⟨#0, λ _ ↦ by simp⟩
 
 lemma bexp_monotone_iff {a i j : M} (hi : i < ‖a‖) (hj : j < ‖a‖) : bexp a i < bexp a j ↔ i < j :=
-  Iff.symm <| Exp.monotone_iff (by simp [hi]) (by simp [hj])
+  Iff.symm <| Exponential.monotone_iff (by simp [hi]) (by simp [hj])
 
 lemma bexp_monotone_le_iff {a i j : M} (hi : i < ‖a‖) (hj : j < ‖a‖) : bexp a i ≤ bexp a j ↔ i ≤ j :=
-  Iff.symm <| Exp.monotone_le_iff (by simp [hi]) (by simp [hj])
+  Iff.symm <| Exponential.monotone_le_iff (by simp [hi]) (by simp [hj])
 
 lemma bexp_eq_of_lt_length {i a a' : M} (ha : i < ‖a‖) (ha' : i < ‖a'‖) : bexp a i = bexp a' i := by
-  have H : Exp i (bexp a i) := by simp [ha]
-  have H' : Exp i (bexp a' i) := by simp [ha']
+  have H : Exponential i (bexp a i) := by simp [ha]
+  have H' : Exponential i (bexp a' i) := by simp [ha']
   exact H.uniq H'
 
 @[simp] lemma bexp_pow2 {a x : M} (h : x < ‖a‖) : Pow2 (bexp a x) := (exp_bexp_of_lt h).range_pow2
@@ -357,9 +357,9 @@ lemma bexp_eq_of_lt_length {i a a' : M} (ha : i < ‖a‖) (ha' : i < ‖a'‖) 
 
 lemma lt_bexp_len {a x : M} (h : ‖x‖ < ‖a‖) : x < bexp a ‖x‖ := lt_exp_len_self (exp_bexp_of_lt h)
 
-lemma bexp_eq_of_exp {a x : M} (h : x < ‖a‖) (H : Exp x y) : bexp a x = y := (exp_bexp_of_lt h).uniq H
+lemma bexp_eq_of_exp {a x : M} (h : x < ‖a‖) (H : Exponential x y) : bexp a x = y := (exp_bexp_of_lt h).uniq H
 
-lemma log_bexp {a x : M} (h : x < ‖a‖) : log (bexp a x) = x := Exp.log_eq_of_exp (exp_bexp_of_lt h)
+lemma log_bexp {a x : M} (h : x < ‖a‖) : log (bexp a x) = x := Exponential.log_eq_of_exp (exp_bexp_of_lt h)
 
 lemma len_bexp {a x : M} (h : x < ‖a‖) : ‖bexp a x‖ = x + 1 := by rw [length_of_pos (bexp_pos h), log_bexp h]
 
@@ -441,7 +441,7 @@ variable [M ⊧ₘ* 𝐈𝚺₁]
 
 @[simp] lemma log_exponential (a : M) : log (exp a) = a := (exp_exponential a).log_eq_of_exp
 
-lemma exponential_log_le_self {a : M} (pos : 0 < a) : exp (log a) ≤ a := by
+lemma exp_log_le_self {a : M} (pos : 0 < a) : exp (log a) ≤ a := by
   rcases log_pos pos with ⟨_, _, H, _⟩
   rcases H.uniq (exp_exponential (log a))
   assumption
@@ -455,7 +455,7 @@ lemma lt_two_mul_exponential_log {a : M} (pos : 0 < a) : a < 2 * exp (log a) := 
   simp [length_of_pos (exp_pos a)]
 
 lemma exp_add (a b : M) : exp (a + b) = exp a * exp b :=
-  exponential_of_exp (Exp.add_mul (exp_exponential a) (exp_exponential b))
+  exp_of_exponential (Exponential.add_mul (exp_exponential a) (exp_exponential b))
 
 lemma log_mul_exp_add_of_lt {a b : M} (pos : 0 < a) (i : M) (hb : b < exp i) : log (a * exp i + b) = log a + i := by
   simp [log_mul_pow2_add_of_lt pos (exp_pow2 i) hb]
@@ -470,7 +470,7 @@ lemma length_mul_exp {a : M} (pos : 0 < a) (i : M) : ‖a * exp i‖ = ‖a‖ +
   simp [length_mul_pow2 pos (exp_pow2 i)]
 
 lemma exp_le_iff_le_log {i a : M} (pos : 0 < a) : exp i ≤ a ↔ i ≤ log a :=
-  ⟨by intro h; simpa using log_monotone h, fun h ↦ le_trans (exponential_monotone_le.mpr h) (exponential_log_le_self pos)⟩
+  ⟨by intro h; simpa using log_monotone h, fun h ↦ le_trans (exp_monotone_le.mpr h) (exp_log_le_self pos)⟩
 
 end ISigma₁
 
