Arithmetization/OmegaOne/Basic.lean
@@ -5,7 +5,7 @@ namespace LO.FirstOrder
 namespace Arith
 
 /-- ∀ x, ∃ y, 2^{|x|^2} = y-/
-def omegaOneAxiom : Sentence ℒₒᵣ := “∀ ∃ ∃[#0 < #2 + 1] (!Model.lengthDef [#0, #2] ∧ !Model.Exp.def [#0*#0, #1])”
+def omegaOneAxiom : Sentence ℒₒᵣ := “∀ ∃ ∃[#0 < #2 + 1] (!Model.lengthDef [#0, #2] ∧ !Model.Exponential.def [#0*#0, #1])”
 
 inductive Theory.omegaOne : Theory ℒₒᵣ where
   | omega : Theory.omegaOne omegaOneAxiom
@@ -21,8 +21,8 @@ namespace Model
 
 variable {M : Type} [Zero M] [One M] [Add M] [Mul M] [LT M]
 
-lemma models_Omega₁_iff [M ⊧ₘ* 𝐈𝚫₀] : M ⊧ₘ omegaOneAxiom ↔ ∀ x : M, ∃ y, Exp (‖x‖^2) y := by
-  simp [models_def, omegaOneAxiom, length_defined.pval, Exp.defined.pval, sq, ←le_iff_lt_succ]
+lemma models_Omega₁_iff [M ⊧ₘ* 𝐈𝚫₀] : M ⊧ₘ omegaOneAxiom ↔ ∀ x : M, ∃ y, Exponential (‖x‖^2) y := by
+  simp [models_def, omegaOneAxiom, length_defined.pval, Exponential.defined.pval, sq, ←le_iff_lt_succ]
   constructor
   · intro h x
     rcases h x with ⟨y, _, _, rfl, h⟩; exact ⟨y, h⟩
@@ -30,7 +30,7 @@ lemma models_Omega₁_iff [M ⊧ₘ* 𝐈𝚫₀] : M ⊧ₘ omegaOneAxiom ↔ �
     rcases h x with ⟨y, h⟩
     exact ⟨y, ‖x‖, by simp, rfl, h⟩
 
-lemma sigma₁_omega₁ [M ⊧ₘ* 𝐈𝚺₁] : M ⊧ₘ omegaOneAxiom := models_Omega₁_iff.mpr (fun x ↦ Exp.range_exists (‖x‖^2))
+lemma sigma₁_omega₁ [M ⊧ₘ* 𝐈𝚺₁] : M ⊧ₘ omegaOneAxiom := models_Omega₁_iff.mpr (fun x ↦ Exponential.range_exists (‖x‖^2))
 
 instance [M ⊧ₘ* 𝐈𝚺₁] : M ⊧ₘ* 𝐈𝚫₀ + 𝛀₁ :=
   ModelsTheory.add_iff.mpr ⟨inferInstance, ⟨by intro _; simp; rintro rfl; exact sigma₁_omega₁⟩⟩
@@ -41,67 +41,67 @@ instance : M ⊧ₘ* 𝐈𝚫₀ := ModelsTheory.of_add_left M 𝐈𝚫₀ 𝛀�
 
 instance : M ⊧ₘ* 𝛀₁ := ModelsTheory.of_add_right M 𝐈𝚫₀ 𝛀₁
 
-lemma exists_exp_sq_length (x : M) : ∃ y, Exp (‖x‖^2) y :=
+lemma exists_exponential_sq_length (x : M) : ∃ y, Exponential (‖x‖^2) y :=
   models_Omega₁_iff.mp (ModelsTheory.models M Theory.omegaOne.omega) x
 
-lemma exists_unique_exp_sq_length (x : M) : ∃! y, Exp (‖x‖^2) y := by
-  rcases exists_exp_sq_length x with ⟨y, h⟩
+lemma exists_unique_exponential_sq_length (x : M) : ∃! y, Exponential (‖x‖^2) y := by
+  rcases exists_exponential_sq_length x with ⟨y, h⟩
   exact ExistsUnique.intro y h (fun y' h' ↦ h'.uniq h)
 
-lemma hash_exists_unique (x y : M) : ∃! z, Exp (‖x‖ * ‖y‖) z := by
+lemma hash_exists_unique (x y : M) : ∃! z, Exponential (‖x‖ * ‖y‖) z := by
   wlog le : x ≤ y
   · simpa [mul_comm] using this y x (le_of_not_ge le)
-  rcases exists_exp_sq_length y with ⟨z, h⟩
+  rcases exists_exponential_sq_length y with ⟨z, h⟩
   have : ‖x‖ * ‖y‖ < ‖z‖ :=
     lt_of_le_of_lt (by simp [sq]; exact mul_le_mul_right (length_monotone le)) h.lt_length
-  have : Exp (‖x‖ * ‖y‖) (bexp z (‖x‖ * ‖y‖)) := exp_bexp_of_lt (a := z) (x := ‖x‖ * ‖y‖) this
+  have : Exponential (‖x‖ * ‖y‖) (bexp z (‖x‖ * ‖y‖)) := exp_bexp_of_lt (a := z) (x := ‖x‖ * ‖y‖) this
   exact ExistsUnique.intro (bexp z (‖x‖ * ‖y‖)) this (fun z' H' ↦ H'.uniq this)
 
 instance : Hash M := ⟨fun a b ↦ Classical.choose! (hash_exists_unique a b)⟩
 
-lemma exp_hash (a b : M) : Exp (‖a‖ * ‖b‖) (a # b) := Classical.choose!_spec (hash_exists_unique a b)
+lemma exponential_hash (a b : M) : Exponential (‖a‖ * ‖b‖) (a # b) := Classical.choose!_spec (hash_exists_unique a b)
 
-lemma exp_hash_one (a : M) : Exp ‖a‖ (a # 1) := by simpa using exp_hash a 1
+lemma exponential_hash_one (a : M) : Exponential ‖a‖ (a # 1) := by simpa using exponential_hash a 1
 
 def hashDef : Δ₀-Sentence 3 :=
-  ⟨“∃[#0 < #2 + 1] ∃[#0 < #4 + 1] (!lengthDef [#1, #3] ∧ !lengthDef [#0, #4] ∧ !Exp.def [#1 * #0, #2])”, by simp⟩
+  ⟨“∃[#0 < #2 + 1] ∃[#0 < #4 + 1] (!lengthDef [#1, #3] ∧ !lengthDef [#0, #4] ∧ !Exponential.def [#1 * #0, #2])”, by simp⟩
 
 lemma hash_defined : Δ₀-Function₂ (Hash.hash : M → M → M) via hashDef := by
-  intro v; simp[hashDef, length_defined.pval, Exp.defined.pval, ←le_iff_lt_succ]
+  intro v; simp[hashDef, length_defined.pval, Exponential.defined.pval, ←le_iff_lt_succ]
   constructor
-  · intro h; exact ⟨‖v 1‖, by simp, ‖v 2‖, by simp, rfl, rfl, by rw [h]; exact exp_hash _ _⟩
-  · rintro ⟨_, _, _, _, rfl, rfl, h⟩; exact h.uniq (exp_hash (v 1) (v 2))
+  · intro h; exact ⟨‖v 1‖, by simp, ‖v 2‖, by simp, rfl, rfl, by rw [h]; exact exponential_hash _ _⟩
+  · rintro ⟨_, _, _, _, rfl, rfl, h⟩; exact h.uniq (exponential_hash (v 1) (v 2))
 
 instance hash_definable : DefinableFunction₂ ℒₒᵣ Σ 0 (Hash.hash : M → M → M) := defined_to_with_param _ hash_defined
 
-@[simp] lemma hash_pow2 (a b : M) : Pow2 (a # b) := (exp_hash a b).range_pow2
+@[simp] lemma hash_pow2 (a b : M) : Pow2 (a # b) := (exponential_hash a b).range_pow2
 
-@[simp] lemma hash_pos (a b : M) : 0 < a # b := (exp_hash a b).range_pos
+@[simp] lemma hash_pos (a b : M) : 0 < a # b := (exponential_hash a b).range_pos
 
-@[simp] lemma hash_lt (a b : M) : ‖a‖ * ‖b‖ < a # b := (exp_hash a b).dom_lt_range
+@[simp] lemma hash_lt (a b : M) : ‖a‖ * ‖b‖ < a # b := (exponential_hash a b).dom_lt_range
 
-lemma length_hash (a b : M) : ‖a # b‖ = ‖a‖ * ‖b‖ + 1 := (exp_hash a b).length_eq
+lemma length_hash (a b : M) : ‖a # b‖ = ‖a‖ * ‖b‖ + 1 := (exponential_hash a b).length_eq
 
-@[simp] lemma hash_zero_left (a : M) : 0 # a = 1 := (exp_hash 0 a).uniq (by simp)
+@[simp] lemma hash_zero_left (a : M) : 0 # a = 1 := (exponential_hash 0 a).uniq (by simp)
 
-@[simp] lemma hash_zero_right (a : M) : a # 0 = 1 := (exp_hash a 0).uniq (by simp)
+@[simp] lemma hash_zero_right (a : M) : a # 0 = 1 := (exponential_hash a 0).uniq (by simp)
 
-lemma hash_comm (a b : M) : a # b = b # a := (exp_hash a b).uniq (by simpa [mul_comm] using exp_hash b a)
+lemma hash_comm (a b : M) : a # b = b # a := (exponential_hash a b).uniq (by simpa [mul_comm] using exponential_hash b a)
 
 @[simp] lemma lt_hash_one_right (a : M) : a < a # 1 := by
-  have : Exp ‖a‖ (a # 1) := by simpa using (exp_hash a 1)
-  exact lt_exp_length this
+  have : Exponential ‖a‖ (a # 1) := by simpa using (exponential_hash a 1)
+  exact lt_exponential_length this
 
 @[simp] lemma lt_hash_one_righs (a : M) : a # 1 ≤ 2 * a + 1 := by
   rcases zero_le a with (rfl | pos)
   · simp
-  · exact (le_iff_lt_length_of_exp (exp_hash a 1)).mpr (by
+  · exact (le_iff_lt_length_of_exp (exponential_hash a 1)).mpr (by
       simp [mul_comm 2 a]
       have : ‖a * 2 + 1‖ = ‖a‖ + 1 := by
         simpa using length_mul_pow2_add_of_lt pos (show Pow2 2 from by simp) one_lt_two
       simp [this])
 
-lemma lt_hash_iff {a b c : M} : a < b # c ↔ ‖a‖ ≤ ‖b‖ * ‖c‖ := (exp_hash b c).lt_iff_len_le
+lemma lt_hash_iff {a b c : M} : a < b # c ↔ ‖a‖ ≤ ‖b‖ * ‖c‖ := (exponential_hash b c).lt_iff_len_le
 
 lemma hash_le_iff {a b c : M} : b # c ≤ a ↔ ‖b‖ * ‖c‖ < ‖a‖ :=
   not_iff_not.mp <| by simp [lt_hash_iff]
@@ -109,14 +109,14 @@ lemma hash_le_iff {a b c : M} : b # c ≤ a ↔ ‖b‖ * ‖c‖ < ‖a‖ :=
 lemma lt_hash_one_iff {a b : M} : a < b # 1 ↔ ‖a‖ ≤ ‖b‖ := by simpa using lt_hash_iff (a := a) (b := b) (c := 1)
 
 lemma hash_monotone {a₁ a₂ b₁ b₂ : M} (h₁ : a₁ ≤ b₁) (h₂ : a₂ ≤ b₂) : a₁ # a₂ ≤ b₁ # b₂ :=
-  (exp_hash a₁ a₂).monotone_le (exp_hash b₁ b₂) (mul_le_mul (length_monotone h₁) (length_monotone h₂) (by simp) (by simp))
+  (exponential_hash a₁ a₂).monotone_le (exponential_hash b₁ b₂) (mul_le_mul (length_monotone h₁) (length_monotone h₂) (by simp) (by simp))
 
-lemma bexp_eq_hash (a b : M) : bexp (a # b) (‖a‖ * ‖b‖) = a # b := bexp_eq_of_exp (by simp [length_hash]) (exp_hash a b)
+lemma bexp_eq_hash (a b : M) : bexp (a # b) (‖a‖ * ‖b‖) = a # b := bexp_eq_of_exp (by simp [length_hash]) (exponential_hash a b)
 
 lemma hash_two_mul (a : M) {b} (pos : 0 < b) : a # (2 * b) = (a # b) * (a # 1) := by
-  have h₁ : Exp (‖a‖ * ‖b‖ + ‖a‖) (a # (2 * b)) := by
-    simpa [length_two_mul_of_pos pos, mul_add] using exp_hash a (2 * b)
-  have h₂ : Exp (‖a‖ * ‖b‖ + ‖a‖) (a # b * a # 1) := (exp_hash a b).add_mul (exp_hash_one a)
+  have h₁ : Exponential (‖a‖ * ‖b‖ + ‖a‖) (a # (2 * b)) := by
+    simpa [length_two_mul_of_pos pos, mul_add] using exponential_hash a (2 * b)
+  have h₂ : Exponential (‖a‖ * ‖b‖ + ‖a‖) (a # b * a # 1) := (exponential_hash a b).add_mul (exponential_hash_one a)
   exact h₁.uniq h₂
 
 lemma hash_two_mul_le_sq_hash (a b : M) : a # (2 * b) ≤ (a # b) ^ 2 := by
