Arithmetization/EA/Basic.lean
@@ -1,0 +1,26 @@
+import Arithmetization.IDeltaZero.Exponential
+
+namespace LO.FirstOrder
+
+namespace Arith
+
+noncomputable section
+
+variable {M : Type} [Nonempty M] [Zero M] [One M] [Add M] [Mul M] [_root_.Exp M] [LT M] [M ⊧ₘ* 𝐄𝐀]
+
+namespace Model
+
+section ISigma₀
+
+variable [M ⊧ₘ* 𝐈𝚺₀]
+
+
+end ISigma₀
+
+end Model
+
+end
+
+end Arith
+
+end LO.FirstOrder
